proving DFA_rlin2

Taskin/DFA_rlin2.thy
@@ -7,18 +7,99 @@ definition nxt_rlin2 :: "('n,'t)Prods \<Rightarrow> 'n \<Rightarrow> 't \<Righta
 "nxt_rlin2 P A a = {B. (A, [Tm a, Nt B]) \<in> P}"
 
 definition nxt_rlin2_set :: "('n,'t)Prods \<Rightarrow> 'n set \<Rightarrow> 't \<Rightarrow> 'n set" where
-"nxt_rlin2_set P M a = (\<Union>A\<in>M. {B. (A, [Tm a, Nt B]) \<in> P})"
+"nxt_rlin2_set P M a = (\<Union>A\<in>M. nxt_rlin2 P A a)"
 
 definition nxts_rlin2_set :: "('n,'t)Prods \<Rightarrow> 'n set \<Rightarrow> 't list \<Rightarrow> 'n set" where
 "nxts_rlin2_set P = foldl (nxt_rlin2_set P)"
 
+lemma nxts_to_mult_derive:
+  "B \<in> nxts_rlin2_set P M w \<Longrightarrow> (\<exists>A\<in>M. P \<turnstile> [Nt A] \<Rightarrow>* map Tm w @ [Nt B])"
+unfolding nxts_rlin2_set_def proof (induction w arbitrary: B rule: rev_induct)
+  case Nil
+  hence 1: "B \<in> M" by simp
+  have 2: "P \<turnstile> [Nt B] \<Rightarrow>* map Tm [] @ [Nt B]" by simp
+  from 1 2 show ?case by blast
+next
+  case (snoc x xs)
+  from snoc.prems have "\<exists>C. C \<in> foldl (nxt_rlin2_set P) M xs \<and> (C, [Tm x, Nt B]) \<in> P"
+    unfolding nxt_rlin2_set_def nxt_rlin2_def by auto
+  then obtain C where C_xs: "C \<in> foldl (nxt_rlin2_set P) M xs" and C_prod: "(C, [Tm x, Nt B]) \<in> P" by blast
+  from C_xs obtain A where A_der: "P \<turnstile> [Nt A] \<Rightarrow>* map Tm xs @ [Nt C]" and A_in: "A \<in> M" 
+    using snoc.IH[of C] by auto
+  from C_prod have "P \<turnstile> [Nt C] \<Rightarrow> [Tm x, Nt B]"
+    using derive_singleton[of P "Nt C" "[Tm x, Nt B]"] by blast
+  hence "P \<turnstile> map Tm xs @ [Nt C] \<Rightarrow> map Tm xs @ [Tm x, Nt B]"
+    using derive_prepend[of P "[Nt C]" "[Tm x, Nt B]" "map Tm xs"] by simp
+  hence C_der: "P \<turnstile> map Tm xs @ [Nt C] \<Rightarrow> map Tm (xs @ [x]) @ [Nt B]" by simp
+  from A_der C_der have "P \<turnstile> [Nt A] \<Rightarrow>* map Tm (xs @ [x]) @ [Nt B]" by simp
+  with A_in show ?case by blast
+qed
+
+lemma rlin2_nts_eq: 
+  assumes "P \<turnstile> [Nt A] \<Rightarrow>* [Nt B]"
+      and "rlin2 P"
+    shows "A = B"
+  sorry
+
+lemma rlin2_intro_tm:
+  assumes "rlin2 P"
+      and "P \<turnstile> [Nt A] \<Rightarrow>* map Tm xs @ [Tm x, Nt B]"
+    shows "\<exists>C. P \<turnstile> [Nt A] \<Rightarrow>* map Tm xs @ [Nt C] \<and> (C,[Tm x, Nt B]) \<in> P"
+  sorry
+
+lemma mult_derive_to_nxts:
+  assumes "rlin2 P"
+  shows "(\<exists>A\<in>M. P \<turnstile> [Nt A] \<Rightarrow>* map Tm w @ [Nt B]) \<Longrightarrow> B \<in> nxts_rlin2_set P M w"
+unfolding nxts_rlin2_set_def using assms proof (induction w arbitrary: B rule: rev_induct)
+  case Nil
+  then obtain A where A_unit: "P \<turnstile> [Nt A] \<Rightarrow>* [Nt B]" and A_in: "A \<in> M" by auto
+  from A_unit Nil.prems(2) have "A = B"
+    using rlin2_nts_eq[of P A B] by simp
+  with A_in show ?case by simp
+next
+  case (snoc x xs)
+  from snoc.prems(1) obtain A where A_der: "P \<turnstile> [Nt A] \<Rightarrow>* map Tm (xs @ [x]) @ [Nt B]" 
+                                and A_in: "A \<in> M" by blast
+  from A_der have "P \<turnstile> [Nt A] \<Rightarrow>* map Tm xs @ [Tm x,Nt B]" by simp
+  with snoc.prems(2) obtain C where C_der: "P \<turnstile> [Nt A] \<Rightarrow>* map Tm xs @ [Nt C]"
+                                and C_prods: "(C,[Tm x, Nt B]) \<in> P" using rlin2_intro_tm by fast
+  from A_in C_der snoc.prems(2) have "C \<in> foldl (nxt_rlin2_set P) M xs"
+    using snoc.IH[of C] by auto
+  with C_prods show ?case
+    unfolding nxt_rlin2_set_def nxt_rlin2_def by auto
+qed
+
+lemma rlin2_fin_eps:
+  assumes "rlin2 P"
+      and "P \<turnstile> [Nt A] \<Rightarrow>* map Tm w"
+    shows "\<exists>B. P \<turnstile> [Nt A] \<Rightarrow>* map Tm w @ [Nt B] \<and> (B,[]) \<in> P"
+  sorry
+
 theorem accepted_if_Lang:
 assumes "rlin2 P"
 shows "w \<in> Lang P A \<Longrightarrow> A \<in> M \<Longrightarrow> \<exists>Z \<in> nxts_rlin2_set P M w. (Z,[]) \<in> P"
-sorry
+proof -
+  assume w_lang: "w \<in> Lang P A" and A_in: "A \<in> M"
+  from assms w_lang obtain B where A_der: "P \<turnstile> [Nt A] \<Rightarrow>* map Tm w @ [Nt B]" and B_in: "(B,[]) \<in> P" 
+    unfolding Lang_def using rlin2_fin_eps by fast
+  from A_in A_der have "B \<in> nxts_rlin2_set P M w" 
+    using mult_derive_to_nxts[OF assms] by auto
+  with B_in show ?thesis by blast
+qed
 
 theorem Lang_if_accepted: "Z \<in> nxts_rlin2_set P M w \<Longrightarrow> (Z,[]) \<in> P \<Longrightarrow> \<exists>A\<in>M. w \<in> Lang P A"
-sorry
+proof -
+  assume Z_nxts: "Z \<in> nxts_rlin2_set P M w" and Z_eps: "(Z,[]) \<in> P"
+  from Z_nxts obtain A where A_der: "P \<turnstile> [Nt A] \<Rightarrow>* map Tm w @ [Nt Z]" and A_in: "A \<in> M"
+    using nxts_to_mult_derive by fast
+  from Z_eps have "P \<turnstile> [Nt Z] \<Rightarrow> []" 
+    using derive_singleton[of P "Nt Z" "[]"] by simp
+  hence "P \<turnstile> map Tm w @ [Nt Z] \<Rightarrow> map Tm w"
+    using derive_prepend[of P "[Nt Z]" "[]" "map Tm w"] by simp
+  with A_der have "P \<turnstile> [Nt A] \<Rightarrow>* map Tm w" by simp
+  with A_in show ?thesis 
+    unfolding Lang_def by blast
+qed
 
 theorem Lang_if_accepted_if_rlin2:
 assumes "rlin2 P"
